Plain old recursive version fully verified

Source/DafnyRuntime/dafnySequence.dfy
@@ -1,20 +1,15 @@
 
-include "../../Test/libraries/src/JSON/Stacks.dfy"
-include "../../Test/libraries/src/Collections/Sequences/Seq.dfy"
 include "../../Test/libraries/src/Math.dfy"
 
 module {:options "/functionSyntax:4"} MetaSeq {
 
   import Math
-  import Seq
-
-  import opened Stacks
 
   datatype SeqExpr<T> = 
     | Empty
     | Direct(a: seq<T>)
     | Concat(left: SeqExpr<T>, right: SeqExpr<T>, length: nat)
-    | Lazy(ghost value: seq<T>, exprBox: AtomicBox<SeqExpr<T>>, length: nat) 
+    | Lazy(ghost value: seq<T>, ghost boxDepth: nat, exprBox: AtomicBox<SeqExpr<T>>, length: nat) 
   {
     ghost predicate Valid()
       decreases Depth(), 0
@@ -24,15 +19,16 @@ module {:options "/functionSyntax:4"} MetaSeq {
         && left.Valid()
         && right.Valid()
         && left.Length() + right.Length() == length
-      case Lazy(value, exprBox, length) => 
+      case Lazy(value, depth, exprBox, length) => 
         && length == |value|
-        && exprBox.inv == ((e: SeqExpr<T>) => e.Valid() && e.Value() == value)
+        && exprBox.inv == ((e: SeqExpr<T>) => e.Depth() < depth && e.Valid() && e.Value() == value)
       case _ => true
     }
 
     ghost function Depth(): nat {
       match this {
         case Concat(left, right, _) => 1 + Math.Max(left.Depth(), right.Depth())
+        case Lazy(_, depth, _, _) => depth
         case _ => 0
       }
     }
@@ -49,7 +45,7 @@ module {:options "/functionSyntax:4"} MetaSeq {
       case Empty => 0
       case Direct(a) => |a|
       case Concat(_, _, length) => length
-      case Lazy(_, _, length) => length
+      case Lazy(_, _, _, length) => length
     }
 
     function At(i: nat): T 
@@ -72,7 +68,7 @@ module {:options "/functionSyntax:4"} MetaSeq {
       case Empty => []
       case Direct(a) => a
       case Concat(left, right, length) => left.Value() + right.Value()
-      case Lazy(value, _, _) => value
+      case Lazy(value, _, _, _) => value
     } by method {
       match this
       case Empty => return [];
@@ -82,7 +78,7 @@ module {:options "/functionSyntax:4"} MetaSeq {
         AppendValue(builder);
         return builder.Value();
       }
-      case Lazy(_, seqExpr, _) => {
+      case Lazy(_, _, seqExpr, _) => {
         var expr := exprBox.Get();
         var value := expr.Value();
         exprBox.Put(Direct(value));
@@ -93,6 +89,7 @@ module {:options "/functionSyntax:4"} MetaSeq {
     method AppendValue(builder: SeqBuilder<T>) 
       requires Valid()
       modifies builder
+      decreases Depth()
       ensures builder.Value() == old(builder.Value()) + Value();
     {
       match this {
@@ -104,120 +101,13 @@ module {:options "/functionSyntax:4"} MetaSeq {
           left.AppendValue(builder);
           right.AppendValue(builder);
         }
-        case Lazy(value, _, _) => {
+        case Lazy(value, _, _, _) => {
           var expr := exprBox.Get();
           expr.AppendValue(builder);
         }
       }
     }
   }
-
-  // function CalcConcatStackBased<T>(left: SeqExpr<T>, right: SeqExpr<T>, length: nat): (result: seq<T>)
-  //   requires left.Valid()
-  //   requires right.Valid()
-  //   requires left.Length() + right.Length() == length
-  //   decreases 1 + Math.Max(left.Depth(), right.Depth())
-  // {
-  //   left.Value() + right.Value()
-  // } by method {
-  //   var builder: SeqBuilder<T> := new SeqBuilder(length);
-  //   assert builder.Value() == [];
-
-  //   var toVisit := new Stack<SeqExpr<T>>(Empty);
-  //   :- expect toVisit.Push(right);
-  //   :- expect toVisit.Push(left);
-  //   assert forall e <- toVisit.Repr :: e.Valid() && e.Depth() < 1 + Math.Max(left.Depth(), right.Depth());
-    
-  //   ghost var answer := left.Value() + right.Value();
-  //   assert toVisit.Repr == [right, left];
-  //   var reversed := Seq.Reverse(toVisit.Repr);
-  //   assert reversed == [left, right];
-  //   assert forall e <- reversed :: e.Valid() && e.Depth() < 1 + Math.Max(left.Depth(), right.Depth());
-  //   ghost var valueFn := (e: SeqExpr<T>) requires e.Valid() => e.Value();
-  //   calc {
-  //     builder.Value() + Seq.Flatten(Seq.Map(valueFn, Seq.Reverse(toVisit.Repr)));
-  //     [] + Seq.Flatten(Seq.Map(valueFn, Seq.Reverse(toVisit.Repr)));
-  //     Seq.Flatten(Seq.Map(valueFn, Seq.Reverse(toVisit.Repr)));
-  //     Seq.Flatten(Seq.Map(valueFn, [left, right]));
-  //     { reveal Seq.Map(); }
-  //     Seq.Flatten([left.Value()] + Seq.Map(valueFn, [right]));
-  //     { reveal Seq.Map(); }
-  //     Seq.Flatten([left.Value(), right.Value()] + []);
-  //     left.Value() + Seq.Flatten([right.Value()]);
-  //     left.Value() + right.Value();
-  //     answer;
-  //   }
-  //   assert builder.Value() + Seq.Flatten(Seq.Map((e: SeqExpr<T>) requires e.Valid() => e.Value(), Seq.Reverse(toVisit.Repr))) == answer;
-
-  //   while 0 < toVisit.size
-  //     invariant toVisit.Valid?()
-  //     invariant fresh(toVisit.data)
-  //     invariant forall e <- toVisit.Repr :: e.Valid() && e.Depth() < 1 + Math.Max(left.Depth(), right.Depth())
-  //     invariant builder.Value() + ConcatValueOnStack(toVisit.Repr) == answer
-  //     decreases TotalNodesOnStack(toVisit.Repr) + TotalDepthOnStack(toVisit.Repr)
-  //   {
-  //     ghost var stackBefore := toVisit.Repr;
-  //     ghost var builderBefore := builder.Value();
-  //     ghost var stackNodesBefore := TotalNodesOnStack(toVisit.Repr);
-  //     ghost var stackDepthBefore :=  TotalDepthOnStack(toVisit.Repr);
-
-  //     // TODO: Have to add Pop() to Stacks.dfy
-  //     var next := toVisit.Pop();
-  //     assert next.Valid();
-
-  //     match next {
-  //       case Concat(nextLeft, nextRight, _) =>
-  //         :- expect toVisit.Push(nextRight);
-  //         :- expect toVisit.Push(nextLeft);
-  //       case _ =>
-  //         assert next.Depth() == 0;
-  //         builder.Append(next.Value());
-  //         assert toVisit.Repr + [next] == stackBefore;
-  //         SumDistributesOverConcat(toVisit.Repr, [next]);
-  //         assert TotalNodesOnStack(toVisit.Repr) + next.NodeCount() == TotalNodesOnStack(stackBefore);
-  //         assert stackNodesBefore < TotalNodesOnStack(toVisit.Repr);
-  //     }
-  //   }
-    
-  //   assert |toVisit.Repr| == 0;
-  //   return builder.Value();
-  // }
-
-  // ghost function ConcatValueOnStack<T>(s: seq<SeqExpr<T>>): seq<T>
-  //   requires (forall e <- s :: e.Valid())
-  // {
-  //   var valueFn := (e: SeqExpr<T>) requires e.Valid() => e.Value();
-  //   Seq.Flatten(Seq.Map(valueFn, Seq.Reverse(s)))
-  // }
-
-  // ghost function TotalDepthOnStack<T>(s: seq<SeqExpr<T>>): nat
-  // {
-  //   Sum(Seq.Map((e: SeqExpr<T>) => e.Depth(), s))
-  // }
-
-  // ghost function TotalNodesOnStack<T>(s: seq<SeqExpr<T>>): nat
-  // {
-  //   Sum(Seq.Map((e: SeqExpr<T>) => e.NodeCount(), s))
-  // }
-
-  // lemma 
-
-  // function Sum(s: seq<nat>): nat {
-  //   Seq.FoldLeft((x, y) => x + y, 0, s)
-  // }
-
-  // lemma SumDistributesOverConcat(a: seq<nat>, b: seq<nat>)
-  //   ensures Sum(a + b) == Sum(a) + Sum(b)
-  // {
-  //   var f := (x, y) => x + y;
-  //   calc {
-  //     Sum(a + b);
-  //     Seq.FoldLeft(f, 0, a + b);
-  //     { Seq.LemmaFoldLeftDistributesOverConcat(f, 0, a, b); }
-  //     Seq.FoldLeft(f, Seq.FoldLeft(f, 0, a), b);
-  //     Sum(a) + Sum(b);
-  //   }
-  // }
 
   // TODO: Make this an extern. How to monomorphize?
   class SeqBuilder<T> {
@@ -240,102 +130,6 @@ module {:options "/functionSyntax:4"} MetaSeq {
       value
     }
   }
-
-  // trait {:termination false} Validatable {
-  //   // Ghost state tracking the common set of objects most
-  //   // methods need to read.
-  //   ghost var Repr: set<object>
-
-  //   ghost predicate Valid()
-  //     reads this, Repr
-  //     ensures Valid() ==> this in Repr
-
-  //   // Convenience predicate for when your object's validity depends on one
-  //   // or more other objects.
-  //   ghost predicate ValidComponent(component: Validatable)
-  //     reads this, Repr 
-  //   {
-  //     && component in Repr
-  //     && component.Repr <= Repr
-  //     && this !in component.Repr
-  //     && component.Valid()
-  //   }
-
-  //   // Convenience predicate, since you often want to assert that 
-  //   // new objects in Repr are fresh as well in most postconditions.
-  //   twostate predicate ValidAndDisjoint()
-  //     reads this, Repr
-  //   {
-  //     Valid() && fresh(Repr - old(Repr))
-  //   }
-  // }
-
-  // // TODO: I THINK this can be a SeqExpr too...
-  // class LazySeq<T> extends Seq<T> {
-  //   const length: nat
-  //   const exprBox: AtomicBox<SeqExpr<T>>
-    
-  //   constructor(expr: SeqExpr<T>) 
-  //     requires expr.Valid()
-  //     ensures Valid()
-  //     ensures this.value == expr.Value()
-  //   {
-  //     this.length := expr.Length();
-  //     this.exprBox := new AtomicBox(expr, ((e: SeqExpr<T>) => e.Valid() && e.Value() == expr.Value()));
-
-  //     this.Repr := {this};
-  //     this.value := expr.Value();
-  //   }
-
-  //   ghost predicate Valid() 
-  //     reads this, Repr
-  //     ensures Valid() ==> this in Repr
-  //   {
-  //     && Repr == {this}
-  //     && length == |value|
-  //     && exprBox.inv == ((e: SeqExpr<T>) => e.Valid() && e.Value() == value)
-  //   }
-
-  //   method Value() returns (s: seq<T>)
-  //     requires Valid()
-  //     ensures s == value
-  //   {
-  //     var expr := Force();
-  //     return expr.Value();
-  //   }
-
-  //   function Length(): nat 
-  //     requires Valid()
-  //     reads Repr
-  //   {
-  //     length
-  //   }
-
-  //   method Concatenate(rhs: Seq<T>) returns (l: Seq<T>) 
-  //     requires Valid() && rhs.Valid()
-  //     ensures l.Valid()
-  //   {
-  //     var expr := exprBox.Get();
-  //     var rhsExpr: SeqExpr<T>;
-  //     if (rhs as Seq<T>) is LazySeq<T> {
-  //       var lazyS := (rhs as Seq<T>) as LazySeq<T>;
-  //       rhsExpr := lazyS.exprBox.Get();
-  //     } else {
-  //       var rhsValue := rhs.Value();
-  //       rhsExpr := Direct(rhsValue);
-  //     }
-  //     var sLength := rhsExpr.Length();
-  //     l := new LazySeq(Concat(expr, rhsExpr, expr.Length() + sLength));
-  //   }
-
-  //   method At(i: nat) returns (t: T) 
-  //     requires Valid()
-  //     requires i < Length()
-  //   {
-  //     var expr := Force();
-  //     return expr.At(i);
-  //   }
-  // }
 
   class {:extern} AtomicBox<T> {
     ghost const inv: T -> bool
